src/SimpleValues.v
@@ -1,0 +1,48 @@
+Require Import Cryptol.AST.
+Require Import Cryptol.Coqlib.
+Require Import Cryptol.Utils. 
+Require Import Omega. 
+
+Section conversion.
+  Variable valtype : Type.
+  Variable isBit : valtype -> option bool.
+  Variable makebit : bool -> valtype.
+
+(* convert Z to bits and back *)
+(* no dependent types this time *)
+Fixpoint to_bitlist (width : nat) (l : list valtype) : option Z :=
+  match l,width with
+  | nil,O => Some 0
+  | f :: r,S n =>
+    match isBit f with
+    | Some b => 
+      match to_bitlist n r with
+      | Some z => Some (z + if b then (two_power_nat n) else 0)
+      | None => None
+      end
+    | _ => None
+    end
+  | _,_ => None
+  end.
+
+Fixpoint from_bitlist (width : nat) (z : Z) : list valtype :=
+  match width with
+  | O => nil
+  | S n' => (makebit (Z.testbit z (Z.of_nat n')) :: from_bitlist n' z)
+  end.
+
+Definition binop (op : Z -> Z -> Z) (width : nat) (a b : list valtype) : option (list valtype) :=
+  match to_bitlist width a, to_bitlist width b with
+  | Some za, Some zb =>
+    Some (from_bitlist width (op za zb))
+  | _ , _ => None
+  end.
+
+(* These are all unsigned operations *)
+Definition add := binop Z.add.
+Definition sub := binop Z.sub.
+Definition mul := binop Z.mul.
+
+End conversion.
+
+
